doc/simple/coq/Subtyping.v
@@ -27,7 +27,7 @@ Admitted.
 Lemma awftyp_pi2: forall G e1 e2 x,
     AWfTyp G (AT_Expr (AE_Pi e1 e2)) ->
     x # G ->
-    AWfTyp (G & x ~ AC_Typ e1) e2.
+    AWfTyp (G & x ~ AC_Typ e1) (e2 @' x).
 Admitted.
 
 Lemma awftyp_forall_evar: forall G e x,
@@ -36,14 +36,832 @@ Lemma awftyp_forall_evar: forall G e x,
     AWfTyp (G & x ~ AC_Unsolved_EVar) (e @@#' (AT_EVar x)).
 Admitted.
 
+Lemma promise_fresh: forall (x:var) L,
+    x \notin L.
+Admitted.
+
+Lemma acpltctxsubst_complete: forall I s t,
+    ok I ->
+    ACpltCtxSubst I s t ->
+    CompleteCtx I.
+Proof.
+  introv oki sub.
+  induction sub; auto.
+  apply~ complete_append. apply~ complete_add_solved.
+  pick_fresh y. assert (y \notin L) by auto.
+  assert (ok (G & y ~ AC_Var)). apply~ ok_push.
+  lets: H0 H1 H2.
+  apply complete_part_left in H3; auto.
+
+  pick_fresh y. assert (y \notin L) by auto.
+  assert (ok (G & y ~ AC_TVar)). apply~ ok_push.
+  lets: H0 H1 H2.
+  apply complete_part_left in H3; auto.
+Qed.
+
 Lemma acpltctxsubst_add_tvar: forall I s t x,
+    AWf I ->
     ACpltCtxSubst I s t ->
     x # I ->
     ACpltCtxSubst (I & x ~ AC_TVar) s t.
 Proof.
+  introv wf sub notin.
+  apply~ a2d_cpltctxsubst.
+  lets: cpltctxsubst_wftyp wf sub.
+  apply~ awtermt_weaken.
+  apply~ complete_add_tvar.
+  lets: acpltctxsubst_complete sub; auto.
+  lets: acpltctxsubst_ctxsubst_a2d wf sub.
+  rewrite~ tsubst_add_tvar.
+Qed.
+
+Fixpoint ASolveCtx (G : ACtx) {struct G} : ACtx :=
+  match G with
+  | nil => nil
+  | cons (x, p) t =>
+    match p with
+    | AC_Unsolved_EVar => ASolveCtx t & x ~ AC_Solved_EVar (AT_Expr AE_Star)
+    | _ => ASolveCtx t & x ~ p
+    end
+  end.
+
+Lemma resolve_evar_awf_preservation: forall G a m s t H,
+    AResolveForall G a m s t H ->
+    AWf G ->
+    AWf H.
+Proof.
+  introv res wf.
+  induction res; auto.
+  assert (AWf (G1 & a1 ~ AC_Unsolved_EVar &
+               a ~ AC_Unsolved_EVar & G2)).
+  rewrite <- concat_assoc.
+  apply~ awf_weakening_insert_unsolved.
+  rewrite~ concat_assoc.
+  lets: IHres H1. auto.
+Qed.
+
+Lemma resolve_forall_extension: forall G a m s t H,
+    AResolveForall G a m s t H ->
+    AWf G ->
+    ExtCtx G H.
+Proof.
+  introv res wfg.
+  lets: resolve_forall_awf_preservation res wfg.
+  lets: awf_is_ok wfg.
+  lets: resolve_forall_wextctx res H1.
+  lets: weak_extension_to_extension H2 wfg H0.
+  auto.
+Qed.
+
+Lemma resolve_forall_inserts2: forall G1 G2 a m e t H,
+    AResolveForall (G1 & a ~ AC_Unsolved_EVar & G2) a m e t H ->
+    ok (G1 & a ~ AC_Unsolved_EVar & G2) ->
+    exists I, H = G1 & I & a ~ AC_Unsolved_EVar & G2 /\
+         (forall a v, binds a v I -> v = AC_Unsolved_EVar).
+Proof.
+  introv res okg. gen_eq S: (G1 & a ~ AC_Unsolved_EVar & G2). gen G1.
+  induction res; introv sinfo; subst; try(solve[exists~ empty]).
+
+  apply ok_middle_eq2 in sinfo; auto.
+  destruct sinfo as [? [? ?]]. subst.
+  assert(ok (G3 & a1 ~ AC_Unsolved_EVar & a ~ AC_Unsolved_EVar & G2)).
+  rewrite <- concat_assoc. apply ok_insert; auto. rewrite~ concat_assoc.
+  forwards*: IHres H1. destruct H3 as (I & [hinfo un]).
+  exists~ (a1 ~ AC_Unsolved_EVar & I).
+  split. repeat rewrite~ concat_assoc.
+  intros n nv bdn.
+  destruct (binds_concat_inv bdn).
+  lets: un H3. auto.
+  destruct H3. apply binds_single_inv in H4. destruct H4. auto.
+  rewrite~ <- sinfo.
+
+  forwards*: IHres1 okg.
+  destruct H0 as (I1 & [h1info bdn]).
+  lets: resolve_forall_ok_preservation res1 okg.
+  lets: IHres2 H0 h1info.
+  destruct H2 as (I2 & [hinfo bdn2]).
+  exists~ (I1 & I2). split. repeat rewrite~ concat_assoc.
+  intros n nv bdnv.
+  destruct (binds_concat_inv bdnv).
+  lets: bdn2 H2. auto.
+  destruct H2. lets: bdn H3. auto.
+
+  forwards*: IHres1 okg.
+  destruct H0 as (I1 & [h1info bdn]).
+  lets: resolve_forall_ok_preservation res1 okg.
+  lets: IHres2 H0 h1info.
+  destruct H2 as (I2 & [hinfo bdn2]).
+  exists~ (I1 & I2). split. repeat rewrite~ concat_assoc.
+  intros n nv bdnv.
+  destruct (binds_concat_inv bdnv).
+  lets: bdn2 H2. auto.
+  destruct H2. lets: bdn H3. auto.
+
+  exists~ (empty: ACtx).
+  split.
+  rewrite~ concat_empty_r.
+  intros n nv bdnv.
+  false binds_empty_inv bdnv.
+Qed.
+
+Lemma actxtsubst_all_unsolved: forall G e,
+    ok G ->
+    (forall a v, binds a v G -> v = AC_Unsolved_EVar) ->
+    ACtxTSubst G e = e.
+Proof.
+  introv okg bd.
+  induction G using env_ind.
+  rewrite~ tsubst_empty_env.
+  assert (binds x v (G & x ~ v)). apply~ binds_push_eq.
+  lets: bd H. subst.
+  rewrite~ tsubst_add_evar.
+  apply~ IHG.
+  intros a v bdav.
+  assert (binds a v (G & x ~ AC_Unsolved_EVar)). apply~ binds_push_neq.
+  introv neq. subst. destruct (ok_push_inv okg).
+  false binds_fresh_inv bdav H1.
+  lets: bd H0. auto.
+Qed.
+
+Lemma resolve_forall_eq_ctxsubst: forall G a m s t H e,
+    AResolveForall G a m s t H ->
+    AWf G ->
+    ACtxTSubst G e = ACtxTSubst H e.
+Proof.
+  introv res wf.
+  induction res; auto.
+
+  assert (AWf (G1 & a1 ~ AC_Unsolved_EVar & a ~ AC_Unsolved_EVar & G2)).
+  rewrite <- concat_assoc.
+  apply~ awf_weakening_insert_unsolved.
+  rewrite~ concat_assoc.
+  lets: IHres H1.
+  do 2 rewrite tsubst_add_ctx in H2.
+  rewrite tsubst_add_evar in H2.
+  do 2 rewrite <- tsubst_add_ctx in H2. auto.
+
+  lets: IHres1 wf.
+  lets: resolve_forall_awf_preservation res1 wf.
+  lets: IHres2 H2.
+  rewrite H3 in H0. auto.
+
+  lets: IHres1 wf.
+  lets: resolve_forall_awf_preservation res1 wf.
+  lets: IHres2 H2.
+  rewrite H3 in H0. auto.
+Qed.
+
+Lemma resolve_forall_eq_g: forall G a m s t H,
+    AResolveForall G a m s t H ->
+    AWf G ->
+    s = ACtxTSubst G s ->
+    t = ACtxTSubst G t.
+Proof.
+  introv res wf sub.
+  induction res; auto.
+  assert (s @@#' AT_EVar a1 =
+          ACtxTSubst (G1 & a1 ~ AC_Unsolved_EVar & a ~ AC_Unsolved_EVar & G2)
+                     (s @@#' AT_EVar a1)).
+  rewrite tsubst_add_ctx.
+  rewrite tsubst_add_ctx.
+  rewrite tsubst_add_evar.
+  do 2 rewrite <- tsubst_add_ctx.
+  rewrite~ actxtsubst_topen.
+  rewrite~ actxtsubst_evar_notin.
+  rewrite actxtsubst_expr in sub.
+  rewrite actxsubst_forall in sub. inversion~ sub.
+  rewrite~ <- H2. rewrite~ <- H2.
+  lets: IHres H1.
+  rewrite <- concat_assoc.
+  apply~ awf_weakening_insert_unsolved.
+  rewrite~ concat_assoc.
+  rewrite tsubst_add_ctx in H2.
+  rewrite tsubst_add_ctx in H2.
+  rewrite tsubst_add_evar in H2.
+  rewrite <- tsubst_add_ctx in H2. rewrite <- tsubst_add_ctx in H2. auto.
+
+  (* PI1 *)
+  rewrite actxtsubst_expr in sub.
+  rewrite actxsubst_pi in sub.
+  inversion~ sub.
+  lets: IHres1 wf H2. clear IHres1.
+
+  lets: resolve_forall_awf_preservation res1 wf.
+  assert (s2 = ACtxTSubst H1 s2).
+  lets: resolve_forall_eq_ctxsubst s2 res1 wf.
+  rewrite~ <- H5.
+  lets: IHres2 H4 H5.
+  lets: resolve_forall_eq_ctxsubst t2 res1 wf.
+
+  rewrite actxtsubst_expr. f_equal.
+  rewrite actxsubst_pi. f_equal~.
+  rewrite <- H7 in H6. auto.
+
+  (* PI2 *)
+  rewrite actxtsubst_expr in sub.
+  rewrite actxsubst_pi in sub.
+  inversion~ sub.
+  lets: IHres1 wf H2. clear IHres1.
+
+  lets: resolve_forall_awf_preservation res1 wf.
+  assert (s2 = ACtxTSubst H1 s2).
+  lets: resolve_forall_eq_ctxsubst s2 res1 wf.
+  rewrite~ <- H5.
+  lets: IHres2 H4 H5.
+  lets: resolve_forall_eq_ctxsubst t2 res1 wf.
+
+  rewrite actxtsubst_expr. f_equal.
+  rewrite actxsubst_pi. f_equal~.
+  rewrite <- H7 in H6. auto.
+Qed.
+
+Lemma resolve_forall_eq_h: forall G a m s t H,
+    AResolveForall G a m s t H ->
+    AWf G ->
+    s = ACtxTSubst G s ->
+    t = ACtxTSubst H t.
+Proof.
+  intros.
+  lets: resolve_forall_eq_g H0 H1 H2.
+  apply resolve_forall_eq_ctxsubst with (e:=t) in H0; auto.
+  rewrite~ <- H0.
+Qed.
+
+Inductive AResolveForall2 : ACtx -> var -> ARFMode -> AType -> AType -> ACtx -> Prop :=
+  | AResolveForall2_Poly: forall a G1 G2 H s t a1,
+      a1 # (G1 & a ~ AC_Unsolved_EVar & G2) ->
+      AResolveForall2 (G1 & a1 ~ AC_Unsolved_EVar & a ~ AC_Unsolved_EVar & G2)
+                     a Plus (s @@#' (AT_EVar a1)) t H ->
+      AResolveForall2 (G1 & a ~ AC_Unsolved_EVar & G2) a Plus (AT_Expr (AE_Forall s)) t H
+  | AResolveForall2_Pi1: forall G s1 s2 t1 t2 H1 H a L,
+      AResolveForall2 G a Plus s1 t1 H1 ->
+      (forall x , x \notin L -> AResolveForall2 (H1 & x ~ AC_Typ s1) a Minus s2 t2 (H & x ~ AC_Typ s1)) ->
+      AResolveForall2 G a Minus (AT_Expr (AE_Pi s1 s2)) (AT_Expr (AE_Pi t1 t2)) H
+  | AResolveForall2_Pi2: forall G s1 s2 t1 t2 H1 H a L,
+      AResolveForall2 G a Minus s1 t1 H1 ->
+      (forall x, x \notin L -> AResolveForall2 (H1 & x ~ AC_Typ s1) a Plus s2 t2 (H & x ~ AC_Typ s1)) ->
+      AResolveForall2 G a Plus (AT_Expr (AE_Pi s1 s2)) (AT_Expr (AE_Pi t1 t2)) H
+  | AResolveForall2_Mono : forall G a m t,
+      ATMono t -> AResolveForall2 G a m t t G.
+
+Hint Constructors AResolveForall2.
+
+Lemma resolve_forall_ok_preservation_inv: forall G a m s t H,
+    AResolveForall G a m s t H ->
+    ok H ->
+    ok G.
+Proof.
+  introv res okh.
+  induction res; auto.
+  lets: IHres okh.
+  rewrite <- concat_assoc.
+  rewrite <- concat_assoc in H1.
+  apply* ok_remove.
+Qed.
+
+Lemma resolve_forall_weakening: forall G a m s t H I,
+    AResolveForall G a m s t H ->
+    ok (H & I) ->
+    AResolveForall (G & I) a m s t (H & I).
+Proof.
+  introv res okg.
+  induction res; auto.
+
+  lets: IHres okg. clear IHres.
+  rewrite <- concat_assoc.
+  apply AResolveForall_Poly with a1; auto.
+  lets: resolve_forall_ok_preservation_inv H1 okg.
+  do 2 rewrite <- concat_assoc in H2.
+  destruct (ok_middle_inv H2). auto.
+  rewrite~ concat_assoc.
+
+  apply AResolveForall_Pi1 with (H1:= (H1 & I)); auto.
+  apply IHres1.
+  lets: IHres2 okg.
+  lets: resolve_forall_ok_preservation_inv H0 okg. auto.
+
+
+  apply AResolveForall_Pi2 with (H1:= (H1 & I)); auto.
+  apply IHres1.
+  lets: IHres2 okg.
+  lets: resolve_forall_ok_preservation_inv H0 okg. auto.
+Qed.
+
+Lemma resolve_forall2_ok_preservation: forall G a m s t H,
+    AResolveForall2 G a m s t H ->
+    ok G -> ok H.
+Proof.
+  introv res okg.
+  induction res; auto.
+  apply IHres.
+  rewrite <- concat_assoc. apply ok_insert. rewrite~ concat_assoc. auto.
+
+  pick_fresh y.
+  assert (y \notin L) by auto.
+  lets: IHres okg.
+  assert (ok (H1 & y ~ AC_Typ s1)) by apply~ ok_push.
+  lets: H2 H3 H5.
+  destruct (ok_push_inv H6). auto.
+
+  pick_fresh y.
+  assert (y \notin L) by auto.
+  lets: IHres okg.
+  assert (ok (H1 & y ~ AC_Typ s1)) by apply~ ok_push.
+  lets: H2 H3 H5.
+  destruct (ok_push_inv H6). auto.
+Qed.
+
+Lemma resolve_forall2_ok_preservation_inv: forall G a m s t H,
+    AResolveForall2 G a m s t H ->
+    ok H -> ok G.
+Proof.
+  introv res okh.
+  induction res; auto.
+  lets: IHres okh.
+  rewrite <- concat_assoc.
+  rewrite <- concat_assoc in H1.
+  apply* ok_remove.
+
+  pick_fresh y.
+  assert (y \notin L) by auto.
+  assert (ok (H & y ~ AC_Typ s1)) by apply~ ok_push.
+  lets: H2 H3 H4.
+  destruct (ok_push_inv H5).
+  lets: IHres H6. auto.
+
+  pick_fresh y.
+  assert (y \notin L) by auto.
+  assert (ok (H & y ~ AC_Typ s1)) by apply~ ok_push.
+  lets: H2 H3 H4.
+  destruct (ok_push_inv H5).
+  lets: IHres H6. auto.
+Qed.
+
+Lemma resolve_forall2_wextctx: forall G a m s t H,
+    AResolveForall2 G a m s t H ->
+    ok G ->
+    WExtCtx G H.
+Proof.
+  introv res okg.
+  lets: resolve_forall2_ok_preservation res okg.
+  induction res; auto.
+
+  (* POLY *)
+  assert(ok (G1 & a1 ~ AC_Unsolved_EVar & a ~ AC_Unsolved_EVar & G2)).
+  rewrite <- concat_assoc.
+  apply ok_insert; auto.
+  rewrite~ concat_assoc.
+  lets: IHres H2 H0.
+  rewrite <- concat_assoc in H3.
+  lets: weak_extension_order_unsolved_evar H3.
+  destruct H4 as (I1 & I2 & [hinfo [g1h1 [? exg2h2]]]).
+  destruct hinfo as [hinfo | (t0 & hinfo)].
+  rewrite hinfo.
+  rewrite <- concat_assoc.
+  apply~ weak_extension_append_ex.
+  apply~ WExtCtx_Add.
+  rewrite hinfo in H0. apply ok_middle_inv_l in H0. auto.
+  rewrite~ concat_assoc.
+  rewrite hinfo in H0; auto.
+  rewrite hinfo.
+  rewrite <- concat_assoc.
+  apply~ weak_extension_append_ex.
+  apply~ WExtCtx_AddSolved.
+  rewrite hinfo in H0. apply ok_middle_inv_l in H0. auto.
+  rewrite~ concat_assoc.
+  rewrite hinfo in H0; auto.
+
+  (* PI1 *)
+  pick_fresh y. assert (y \notin L) by auto.
+  lets: H2 H4. clear H2.
+  lets: resolve_forall2_ok_preservation res okg.
+  lets: IHres okg H2. clear IHres.
+  assert (ok (H1 & y ~ AC_Typ s1)) by apply~ ok_push.
+  assert (ok (H & y ~ AC_Typ s1)) by apply~ ok_push.
+  lets: H3 H4 H7 H8.
+  lets: weak_extension_remove_typvar H9.
+  lets: weak_extension_transitivity H6 H10. auto.
+
+  (* PI2 *)
+  pick_fresh y. assert (y \notin L) by auto.
+  lets: H2 H4. clear H2.
+  lets: resolve_forall2_ok_preservation res okg.
+  lets: IHres okg H2. clear IHres.
+  assert (ok (H1 & y ~ AC_Typ s1)) by apply~ ok_push.
+  assert (ok (H & y ~ AC_Typ s1)) by apply~ ok_push.
+  lets: H3 H4 H7 H8.
+  lets: weak_extension_remove_typvar H9.
+  lets: weak_extension_transitivity H6 H10. auto.
+Qed.
+
+Lemma weak_extension_var_preservation_inv: forall G H x,
+    WExtCtx G H ->
+    x # H -> x # G.
+Proof.
+  introv ex.
+  induction ex; auto.
+Qed.
+
+Lemma resolve_forall2_renaming: forall x y G1 G2 t1 t2 H1 H2 a m s t,
+    x <> y ->
+    ok (G1 & x ~ AC_Typ t1 & G2) ->
+    ok (H1 & y ~ AC_Typ t1 & H2) ->
+    AResolveForall2 (G1 & x ~ AC_Typ t1 & G2) a m s t (H1 & x ~ AC_Typ t1 & H2) ->
+    AResolveForall2 (G1 & y ~ AC_Typ t1 & G2) a m s t (H1 & y ~ AC_Typ t2 & H2).
+Proof.
+  introv neq okx oky res.
+  assert (ok (G1 & y ~ AC_Typ t1 & G2)).
+  apply ok_insert; auto.
+  destruct (ok_middle_inv oky).
+  assert (y # (H1 & x ~ AC_Typ t1 & H2)). auto.
+  lets: resolve_forall2_wextctx res okx.
+  lets: weak_extension_var_preservation_inv H4 H3. auto.
+
+  gen_eq S: (G1 & x ~ AC_Typ t1 & G2).
+  gen_eq M: (H1 & x ~ AC_Typ t1 & H2). gen G1 G2 H1 H2.
+  induction res; introv okyg okyh minfo sinfo; subst; auto.
+
+  admit.
+
+  lets: resolve_forall2_ok_preservation res okx.
+  lets: resolve_forall2_wextctx res okx.
+  lets: weak_extension_order_typvar H5.
+  destruct H6 as (I1 & I2 & [h1info _]). subst.
+  forwards ~ : IHres okx okyg I1 I2.
+
+
+  apply ok_middle
+
+Lemma resolve_forall2_weakening: forall x y G1 G2 t1 t2 H1 H2 a m s t,
+    x <> y ->
+    ok (G1 & x ~ AC_Typ t1 & y ~ AC_Typ t2 & G2) ->
+    AResolveForall2 (G1 & x ~ AC_Typ t1 & y ~ AC_Typ t2 & G2) a m s t (H1 & x ~ AC_Typ t1 & y ~ AC_Typ t2 & H2) ->
+    AResolveForall2 (G1 & y ~ AC_Typ t2 & x ~ AC_Typ t2 & G2) a m s t (H1 & y ~ AC_Typ t2 & x ~ AC_Typ t1 & H2).
+Proof.
+  introv neq okg res.
+  gen_eq S: (G1 & x ~ AC_Typ t1 & y ~ AC_Typ t2 & G2).
+  gen_eq M: (H1 & x ~ AC_Typ t1 & y ~ AC_Typ t2 & H2).
+  gen G1 G2 H1 H2.
+  induction res; introv minfo sinfo; subst.
+
+  admit.
+
+  lets: resolve_forall2_wextctx res okg.
+  lets: weak_extension
+
+  admit.
+
+  lets: resolve_forall2_wextctx res.
+
+
+  apply IHres.
+  introv neq res.
+  inductions res; auto.
+
+  assert (ok (G1 & a1 ~ AC_Unsolved_EVar & a ~ AC_Unsolved_EVar & G2)).
+  rewrite <- concat_assoc. apply ok_insert; auto.
+  rewrite~ concat_assoc.
+  lets: resolve_forall2_ok_preservation res H.
+  lets: IHres H. clear IHres.
+
+
+Lemma resolve_forall2_weakening: forall G a m s t H y v,
+    AResolveForall2 G a m s t H ->
+    ok (H & y ~ AC_Typ v) ->
+    AResolveForall2 (G & y ~ AC_Typ v) a m s t (H & y ~ AC_Typ v).
+Proof.
+  introv res okh.
+  induction res; auto.
+  rewrite <- concat_assoc.
+  destruct (ok_push_inv okh).
+  lets: IHres okh. clear IHres.
+  apply AResolveForall2_Poly with a1; auto.
+  lets: resolve_forall2_ok_preservation_inv H3 okh.
+  do 2 rewrite <- concat_assoc in H4.
+  destruct (ok_middle_inv H4). auto.
+  repeat rewrite~ concat_assoc in H3.
+  repeat rewrite~ concat_assoc.
+
+  apply AResolveForall2_Pi1 with (H1:=H1 & y ~ AC_Typ v) (L:= L \u dom H \u dom H1 \u \{y}).
+  pick_fresh z. assert (z \notin L) by auto.
+  assert (ok (H & z ~ AC_Typ s1 & y ~ AC_Typ v)). apply ok_insert; auto.
+  lets: H2 H3 H4. clear H2.
+  lets: resolve_forall2_ok_preservation_inv H5 H4.
+  lets: ok_remove H2.
+  lets: IHres H6. auto.
+
+  intros z notin.
+  assert (z \notin L) by auto.
+  assert (ok (H & z ~ AC_Typ s1 & y ~ AC_Typ v)). apply ok_insert; auto.
+  lets: H2 H3 H4.
+
+Lemma resolve_forall2_weakening: forall G1 G2 a m s t H I,
+    AResolveForall2 (G1 & G2) a m s t H ->
+    ok (H & I) ->
+    exists H1 H2, H = H1 & H2 /\ AResolveForall2 (G1 & I & G2) a m s t (H1 & I & H2).
+Proof.
+  introv res okg. gen_eq S: (G1 & G2). gen G1 G2.
+  induction res; introv sinfo; subst; auto.
+
+  (* POLY *)
+  assert (ok H). destruct (ok_concat_inv okg). auto.
+  assert (ok (G1 & a1 ~ AC_Unsolved_EVar & a ~ AC_Unsolved_EVar & G2)).
+  lets: resolve_forall2_ok_preservation_inv res H1. auto.
+  assert (ok (G1 & a ~ AC_Unsolved_EVar & G2)).
+  rewrite <- concat_assoc in H2.
+  lets: ok_remove H2.
+  rewrite~ <- concat_assoc.
+  assert (binds a AC_Unsolved_EVar (G0 & G3)).
+  rewrite <- sinfo. apply~ binds_middle_eq.
+  destruct (ok_middle_inv H3). auto.
+
+  destruct (binds_concat_inv H4).
+  apply split_bind_context in H5.
+  destruct H5 as (M1 & M2 & g3info). subst.
+  repeat rewrite concat_assoc in sinfo.
+  apply ok_middle_eq2 in sinfo; auto.
+  destruct sinfo as [? [_ ?]]. subst.
+  assert (G0 & M1 & a1 ~ AC_Unsolved_EVar & a ~ AC_Unsolved_EVar & M2 =
+          G0 & (M1 & a1 ~ AC_Unsolved_EVar & a ~ AC_Unsolved_EVar & M2)).
+  repeat rewrite~ concat_assoc.
+  lets: IHres okg H5. clear IHres.
+  destruct H6 as (M3 & M4 & [hinfo res2]). subst.
+  exists~ M3 M4. split~.
+  repeat rewrite concat_assoc in *.
+  apply AResolveForall2_Poly with (a1:=a1); auto.
+  assert (ok (M3 & I & M4)).
+  admit.
+  lets: resolve_forall2_ok_preservation_inv res2 H.
+  rewrite <- concat_assoc in H6.
+  destruct (ok_middle_inv H6). auto.
+  rewrite~ <- sinfo.
+
+  destruct H5.
+  apply split_bind_context in H6.
+  destruct H6 as (M1 & M2 & g0info). subst.
+  assert (sinfo' : G1 & a ~ AC_Unsolved_EVar & G2 = M1 & a ~ AC_Unsolved_EVar & (M2 & G3)).
+  repeat rewrite~ concat_assoc.
+  apply ok_middle_eq2 in sinfo'; auto.
+  destruct sinfo' as [? [_ ?]]. subst.
+  assert (M1 & a1 ~ AC_Unsolved_EVar & a ~ AC_Unsolved_EVar & (M2 & G3) =
+          (M1 & a1 ~ AC_Unsolved_EVar & a ~ AC_Unsolved_EVar & M2) & G3).
+  repeat rewrite~ concat_assoc.
+  lets: IHres okg H6. clear IHres.
+  destruct H7 as (M3 & M4 & [hinfo res2]). subst.
+  exists~ M3 M4. split~.
+  assert (AResolveForall2
+           (M1 & a1 ~ AC_Unsolved_EVar & a ~ AC_Unsolved_EVar & (M2 & I & G3)) a
+           Plus (s @@#' AT_EVar a1) t (M3 & I & M4)).
+  repeat rewrite~ concat_assoc.
+  lets: AResolveForall2_Poly H.
+  assert (ok (M3 & I & M4)).
+  admit.
+  lets: resolve_forall2_ok_preservation_inv res2 H7.
+  do 3 rewrite <- concat_assoc in H8.
+  destruct (ok_middle_inv H8). auto.
+  repeat rewrite concat_assoc in H7. auto.
+  rewrite~ <- sinfo'.
+
+  (* PI1 *)
+  pick_fresh y. assert (y \notin L) by auto.
+  lets: H0 H3. clear H0.
+  assert (ok (H & y ~ AC_Typ s1)). apply~ ok_push.
+  lets: resolve_forall2_ok_preservation_inv H4 H0.
+  assert (ok (H1 & I)). admit.
+  forwards *: IHres H6.
+  destruct H7 as (M1 & M2 & [h1info res2]). subst.
+  assert (ok (H & y ~ AC_Typ s1 & I)). apply ok_insert; auto.
+  assert (M1 & M2 & y ~ AC_Typ s1 =
+          M1 & (M2 & y ~ AC_Typ s1)). repeat rewrite~ concat_assoc.
+  lets: H2 H3 H1 H7.
+  destruct H8 as (M3 & M4 & [hinfo  res3]).
+  assert (binds y (AC_Typ s1) (M3 & M4)).
+  rewrite <- hinfo. apply~ binds_push_eq.
+  destruct (binds_concat_inv H8).
+  apply split_bind_context in H9.
+  destruct H9 as (M5 & M6 & m4info). subst.
+  symmetry in hinfo.
+  repeat rewrite concat_assoc in *.
+  apply tail_empty_eq2 in hinfo; auto.
+  destruct hinfo as [? [_ ?]]. subst.
+  repeat rewrite concat_empty_r in *.
+  exists~ M3 M5. split; auto.
+  apply AResolveForall2_Pi1 with (H1:=(M1 & I & M2))
+         (L:=(((((((((L \u \{ a}) \u ATFv s1) \u ATFv s2) \u ATFv t1) \u ATFv t2) \u dom I) \u dom (M1 & M2)) \u dom (M3 & M5)) \u dom G1)); auto.
+  intros z notinz.
+  admit.
+  rewrite~ hinfo.
+
+  destruct H9.
+  apply split_bind_context in H10.
+  destruct H10 as (M5 & M6 & m4info). subst.
+  symmetry in hinfo. rewrite <- concat_assoc in hinfo.
+  apply tail_empty_eq2 in hinfo; auto.
+  destruct hinfo as [? [_ ?]]. symmetry in H11. lets: empty_concat_inv H11. destruct H12. subst.
+  repeat rewrite concat_empty_r in *.
+  assert (I = empty).
+  induction I using env_ind; auto. clear IHI.
+  repeat rewrite concat_assoc in *.
+  assert (AResolveForall2 (M1 & I & x ~ v & M2 & y ~ AC_Typ s1 & empty) a Minus s2 t2
+                          (M5 & y ~ AC_Typ s1 & I & x ~ v & empty)).
+  repeat rewrite~ concat_empty_r.
+  assert (ok (M1 & I & x ~ v & M2 & y ~ AC_Typ s1 & empty)). repeat rewrite~ concat_empty_r. lets: resolve_forall2_ok_preservation_inv res3 H1. auto.
+  lets: resolve_forall2_wextctx H H10.
+  forwards*: weak_declaration_order_preservation H12.
+  destruct H13 as (? & ? & ? & ? & ? &?).
+  lets: reverse_order_inv H13; auto.
+  rewrite~ concat_empty_r.
+  rewrite <- H13. rewrite~ concat_empty_r. false H14.
+
+  subst.
+  exists~ M5 (empty: ACtx).
+  repeat rewrite concat_empty_r in *. split; auto.
+  repeat rewrite concat_assoc in *.
+  apply AResolveForall2_Pi1 with (H1:=(M1 & M2))
+         (L:=(((((((((L \u \{ a}) \u ATFv s1) \u ATFv s2) \u ATFv t1) \u ATFv t2) \u dom (M1 & M2)) \u dom (M5)) \u dom G1))); auto.
+  intros z notinz.
+
+  admit.
+  rewrite~ hinfo.
+
+  admit.
+
+  exists~ G1 G2.
+Qed.
+
+Lemma resolve_is_resolve2: forall G a m s t H,
+    AResolveForall G a m s t H ->
+    AResolveForall2 G a m s t H.
+Proof.
+  introv res.
+  induction res; auto.
+  apply~ AResolveForall2_Poly.
+
+  apply AResolveForall2_Pi1 with (H1:=H1) (L:=dom H); auto.
+  intros y notin.
+  apply~ resolve_forall_weakening.
+       apply~ resolve_forall_Weakening
+
+
+Lemma resolve_forall_awftyp_preservation: forall G a m s t H,
+    AResolveForall G a m s t H ->
+    AWfTyp G s ->
+    AWfTyp H t.
+Proof.
+  introv res wf.
+  induction res; auto.
+  admit.
+
+  lets: awftyp_pi1 wf.
+  lets: IHres1 H0.
+  lets: awftyp_awf wf.
+  lets: resolve_forall_extension res1 H3.
+  lets: awftyp_pi2 wf.
 Admitted.
 
-Theorem subtype_soundness: forall G H I t1 t2 H' t1' t2',
+Lemma subtyping_extension: forall G t s H,
+    ASubtyping G t s H ->
+    AWf G ->
+    AWfTyp G t ->
+    AWfTyp G s ->
+    t = ACtxTSubst G t ->
+    s = ACtxTSubst G s ->
+    AWf H /\ ExtCtx G H.
+Proof.
+  introv sub wfg wtt wts subt subs.
+  induction sub.
+
+  (* POLYR *)
+  assert (I1: AWf (G & v ~ AC_TVar)). apply~ AWf_TVar.
+  assert (I2: AWfTyp (G & v ~ AC_TVar) s1). apply~ awftyp_weakening.
+  assert (I3: AWfTyp (G & v ~ AC_TVar) (s2 @@#' AT_TFVar v)). apply~ awftyp_forall.
+  assert (I4: s1 = ACtxTSubst (G & v ~ AC_TVar) s1). rewrite~ tsubst_add_tvar.
+  assert (I5: s2 @@#' AT_TFVar v = ACtxTSubst (G & v ~ AC_TVar) (s2 @@#' AT_TFVar v)).
+  rewrite tsubst_add_tvar.
+  rewrite~ actxtsubst_topen. rewrite~ actxtsubst_tfvar_notin.
+  rewrite actxtsubst_expr in subs.
+  rewrite actxsubst_forall in subs.
+  inversion~ subs. rewrite~ <- H2. rewrite~ <- H2.
+  lets: IHsub I1 I2 I3 I4 I5.
+  destruct H1.
+  split. lets: AWf_left H1. auto.
+  lets: extension_remove_tvar H2. auto.
+
+  (* POLYL *)
+  assert (I1: AWf (G & b ~ AC_Marker & a ~ AC_Unsolved_EVar)).
+  apply~ AWf_Ctx_Unsolved_EVar.
+  assert (I2: AWfTyp (G & b ~ AC_Marker & a ~ AC_Unsolved_EVar)
+                     (s1 @@#' AT_EVar a)).
+  apply~ awftyp_forall_evar.
+  apply~ awftyp_weakening.
+  assert (I3: AWfTyp (G & b ~ AC_Marker & a ~ AC_Unsolved_EVar) s2).
+  apply~ awftyp_weakening.
+  apply~ awftyp_weakening.
+  assert (I4: s1 @@#' AT_EVar a =
+              ACtxTSubst (G & b ~ AC_Marker & a ~ AC_Unsolved_EVar)
+                         (s1 @@#' AT_EVar a)).
+  rewrite tsubst_add_evar.
+  rewrite tsubst_add_marker.
+  rewrite~ actxtsubst_topen.
+  rewrite~ actxtsubst_evar_notin.
+  rewrite actxtsubst_expr in subt.
+  rewrite actxsubst_forall in subt.
+  inversion~ subt. repeat rewrite~ <- H4.
+  assert (I5: s2 = ACtxTSubst (G & b ~ AC_Marker & a ~ AC_Unsolved_EVar) s2).
+  rewrite tsubst_add_evar.
+  rewrite~ tsubst_add_marker.
+  lets: IHsub I1 I2 I3 I4 I5.
+  destruct H3.
+  split. do 2 apply AWf_left in H3. auto.
+  lets: extension_order_marker H4.
+  destruct H5 as (M1 & M2 & [hinfo [gh1 _]]).
+  apply ok_middle_eq2 in hinfo; auto.
+  destruct hinfo as [? [? ?]]. rewrite~ H5.
+  rewrite~ <- hinfo.
+
+  (* PI *)
+  rewrite actxtsubst_expr in subt.
+  rewrite actxsubst_pi in subt.
+  rewrite actxtsubst_expr in subs.
+  rewrite actxsubst_pi in subs.
+  destruct IHsub1; auto. apply awftyp_pi1 in wts; auto.
+  apply awftyp_pi1 in wtt; auto.
+  inversion~ subs. rewrite~ <- H3.
+  inversion~ subt. rewrite~ <- H3.
+
+  assert (I1: AWf (H1 & x ~ AC_Typ s1)).
+  apply~ AWf_TyVar. apply awftyp_pi1 in wtt.
+  lets: extension_weakening_awftyp wtt H3. auto.
+  assert (I2: AWfTyp (H1 & x ~ AC_Typ s1)
+                     (ACtxTSubst H1 (s2 @@' AE_FVar x))).
+  rewrite <- tsubst_add_typvar with (x:=x) (t:=s1).
+  apply -> awftyp_subst.
+  assert (x # G). lets: declaration_preservation_inv H3 H0. auto.
+  lets: awftyp_pi2 wtt H4.
+  assert (ExtCtx (G & x ~ AC_Typ s1) (H1 & x ~ AC_Typ s1)).
+  apply~ ExtCtx_TypVar.
+  apply~ AWf_TyVar. apply awftyp_pi1 in wtt; auto.
+  lets: extension_weakening_awftyp H5 H6. auto.
+  assert (I3: AWfTyp (H1 & x ~ AC_Typ s1) (ACtxTSubst H1 (s4 @@' AE_FVar x))).
+  admit.
+  assert (I4: ACtxTSubst H1 (s2 @@' AE_FVar x) =
+              ACtxTSubst (H1 & x ~ AC_Typ s1)
+                         (ACtxTSubst H1 (s2 @@' AE_FVar x))).
+  rewrite tsubst_add_typvar.
+  rewrite~ ctxtsubst_twice.
+  assert (I5: ACtxTSubst H1 (s4 @@' AE_FVar x) =
+              ACtxTSubst (H1 & x ~ AC_Typ s1)
+                         (ACtxTSubst H1 (s4 @@' AE_FVar x))).
+  rewrite tsubst_add_typvar.
+  rewrite~ ctxtsubst_twice.
+  lets: IHsub2 I1 I2 I3 I4 I5.
+  destruct H4.
+
+  split. lets: AWf_left H4. auto.
+  lets: extension_remove_tyvar H5.
+  lets: extension_transitivity H3 H6. auto.
+
+  (* EVARL *)
+  lets: resolve_forall_extension H2 wfg.
+  lets: resolve_forall_awf_preservation H2 wfg.
+
+  assert (I1: t = ACtxTSubst H1 t).
+  lets: resolve_forall_eq_h H2 wfg subs. auto.
+  assert (I2: AT_EVar a = ACtxTSubst H1 (AT_EVar a)).
+  lets: resolve_forall_eq_ctxsubst (AT_EVar a) H2 wfg.
+  rewrite H6 in subt. auto.
+  assert (I3: AWfTyp H1 t).
+  lets: resolve_forall_awftyp_preservation H2 wts. auto.
+  assert (I4: AWfTyp H1 (AT_EVar a)).
+  lets: extension_weakening_awftyp wtt H4. auto.
+  forwards: unify_extension H3 H5 I1 I2 I3. auto.
+  destruct H6.
+  split; auto.
+  lets: extension_transitivity H4 H7. auto.
+
+  (* EVARR *)
+  lets: resolve_forall_extension H2 wfg.
+  lets: resolve_forall_awf_preservation H2 wfg.
+
+  assert (I1: t = ACtxTSubst H1 t).
+  lets: resolve_forall_eq_h H2 wfg subt. auto.
+  assert (I2: AT_EVar a = ACtxTSubst H1 (AT_EVar a)).
+  lets: resolve_forall_eq_ctxsubst (AT_EVar a) H2 wfg.
+  rewrite H6 in subs. auto.
+  assert (I3: AWfTyp H1 t).
+  lets: resolve_forall_awftyp_preservation H2 wtt. auto.
+  assert (I4: AWfTyp H1 (AT_EVar a)).
+  lets: extension_weakening_awftyp wts H4. auto.
+  forwards: unify_extension H3 H5 I1 I2 I3. auto.
+  destruct H6.
+  split; auto.
+  lets: extension_transitivity H4 H7. auto.
+
+  (* UNIFY *)
+  forwards: unify_extension H0; auto.
+Qed.
+
+Theorem subtyping_soundness: forall G H I t1 t2 H' t1' t2',
     ASubtyping G t1 t2 H ->
     t1 = ACtxTSubst G t1 ->
     t2 = ACtxTSubst G t2 ->
@@ -95,6 +913,7 @@ Proof.
   apply~ complete_add_tvar.
   assert (I8: ACpltCtxSubst (I & v ~ AC_TVar) s1 t1').
   apply~ acpltctxsubst_add_tvar.
+  lets: awf_preservation H4. auto.
   lets: promise_fresh v (dom I). auto.
   assert(I9: ACpltCtxSubst (I & v ~ AC_TVar) (s2 @@#' AT_TFVar v) (s3 ^^%' DT_TFVar v)).
   lets: promise_fresh v L.
@@ -133,8 +952,46 @@ Proof.
   assert (I5: AWfTyp (G & b ~ AC_Marker & a ~ AC_Unsolved_EVar) s2).
   apply* awftyp_weakening.
   apply* awftyp_weakening.
+  lets: IHASubtyping I1 I2 I3 I4 I5. clear IHASubtyping.
+  lets: awf_is_ok I3.
+  lets: subtyping_ok_preservation H3 H15.
 
-  admit.
+  assert (Softness I).
+  forwards ~ : subtyping_wextctx H3.
+  lets: weak_extension_order_marker H18.
+  destruct H19 as (M1 & M2 & [hinfo [_ [sf _]]]).
+  apply ok_middle_eq2 in hinfo; auto.
+  destruct hinfo as [? [_ ?]]. rewrite H20.
+  apply~ sf. apply soft_single_unsolved.
+  rewrite~ <- hinfo.
+
+  assert (binds a AC_Unsolved_EVar (G & b ~ AC_Marker & a ~ AC_Unsolved_EVar)). apply~ binds_push_eq.
+  forwards: subtyping_evar_preservation H3 H19; auto.
+  destruct H20 as [bdun | (ta & bdso)].
+
+  (* a is unsolved in I *)
+  assert (a # (H & b ~ AC_Marker)).
+  lets: subtyping_wextctx H3 H15.
+  assert ((G & b ~ AC_Marker & a ~ AC_Unsolved_EVar) = (G & b ~ AC_Marker & empty & a ~ AC_Unsolved_EVar & empty)) by repeat rewrite~ concat_empty_r.
+  lets: weak_declaration_order_preservation H20 H21.
+  destruct H22 as (? & ? & ? & ? & ? & ?).
+  assert( H & b ~ AC_Marker & I =
+          x1 & b ~ x & (x2 & a ~ x0 & x3)) by repeat rewrite~ concat_assoc.
+  apply ok_middle_eq2 in H23; auto.
+  destruct H23 as [? [? ?]]. rewrite H23 in *.
+  rewrite H22 in H17. apply ok_middle_inv_l in H17. auto.
+  rewrite~ <- H23.
+
+  assert (I6: ExtCtx (H & b ~ AC_Marker & I)
+                     (I0 & b ~ AC_Marker & I)).
+  apply~ extension_append.
+  apply~ ExtCtx_Marker.
+  assert (I6: ExtCtx (H & b ~ AC_Marker & I)
+                     (I0 & b ~ AC_Marker & (ASolveCtx I))).
+
+  lets: binds_concat_right_inv bdun H20. clear bdun H20.
+
+
 
   (* PI *)
   inversion H6; subst.
@@ -148,16 +1005,35 @@ Proof.
   lets: IHASubtyping1 H18 H13 H8 H21 H12. clear IHASubtyping1 H14 H20 H17 H19.
   admit.
 
-  (* EVARL *)
   admit.
+
+  (* EVARL *)
+  lets: resolve_forall_awf_preservation H2 H8.
+  inversion H2; subst.
+
+  (* resolve pi *)
+  inversion H12; subst.
+  admit.
+
+  (* resolve mono *)
+  forwards ~ : unif_soundness_same H3 H6 H13 H11 H12.
+  rewrite H1. apply DSub_AEq.
 
   (* EVARR *)
+  lets: resolve_forall_awf_preservation H2 H8.
+  inversion H2; subst.
+
+  (* resolve forall *)
+  false H0. reflexivity.
+
+  (* resolve pi *)
   admit.
 
+  (* resolve mono *)
+  forwards ~ : unif_soundness_same H3 H6 H13 H12 H11.
+  rewrite H1. apply DSub_AEq.
+
   (* UNIFY *)
-  lets: unif_soundness_same H0 H1 H2 H3 H4.
-  lets: H11 H5 H6 H7 H8. clear H11.
-  lets: awtermt_awftyp H9.
-  lets: awtermt_awftyp H10.
-  lets: H12 H11 H13.
-  rewrite H14. apply DSub_AEq.
+  forwards * : unif_soundness_same H0 H5 H6 H7.
+  rewrite H11. apply DSub_AEq.
+Qed.
