doc/simple/coq/UtilityTyping.v
@@ -1,0 +1,172 @@
+Require Import LibLN.
+Require Import DeclDef.
+Require Import DeclInfra.
+Require Import AlgoDef.
+Require Import AlgoInfra.
+Require Import CtxExtension.
+Require Import UtilityEnv.
+Require Import Subst.
+Require Import Exists.
+Require Import UtilityMore.
+Require Import WeakExtension.
+Require Import UtilityAlgo.
+
+(* CONTEXT EQUAL UP TO RENAMING *)
+
+Lemma typing_insert_unsolved_evar: forall G1 G2 m e t H a,
+    ATyping m (G1 & G2) e t H ->
+    a # (G1 & G2) ->
+    exists I I1 I2 H2, ATyping m (G1 & a ~ AC_Unsolved_EVar & G2) e t I
+                  /\ I = I1 & a ~ AC_Unsolved_EVar & I2
+                  /\ H = I1 & H2
+                  (*/\ I2 H2 has ....*)
+
+with awf_insert_unsolved_evar: forall G1 G2 a,
+    AWf (G1 & G2) ->
+    a # (G1 & G2) ->
+    AWf (G1 & a ~ AC_Unsolved_EVar & G2).
+Proof.
+  introv ty notin. gen_eq G:(G1 & G2). gen G1 G2.
+  lets: atyping_awf ty.
+  induction ty; introv ginfo; subst; auto.
+
+  admit.
+
+
+
+  exists~ (G1 & a ~ AC_Unsolved_EVar & G2).
+  (* VAR *)
+  exists~ (G1 & a ~ AC_Unsolved_EVar & G2). apply ATI_Var. apply* awf_insert_unsolved_evar.
+  assert (a <> x). introv neq; subst. false binds_fresh_inv H1 notin0.
+  apply~ binds_weaken.
+
+  (* EVAR *)
+  exists~ (G1 & a ~ AC_Unsolved_EVar & G2). apply ATI_EVar. apply* awf_insert_unsolved_evar.
+  assert (a <> x). introv neq; subst. false binds_fresh_inv H1 notin0.
+  apply~ binds_weaken.
+
+  (* EVAR *)
+  exists~ (G1 & a ~ AC_Unsolved_EVar & G2). apply ATI_Solved_EVar with t. apply* awf_insert_unsolved_evar.
+  assert (a <> x). introv neq; subst. false binds_fresh_inv H1 notin0.
+  apply~ binds_weaken.
+
+  (* TVar *)
+  exists~ (G1 & a ~ AC_Unsolved_EVar & G2). apply ATI_TVar. apply* awf_insert_unsolved_evar.
+  assert (a <> x). introv neq; subst. false binds_fresh_inv H1 notin0.
+  apply~ binds_weaken.
+
+  (* ANN *)
+
+(* Lemma unify_same: forall G a, *)
+(*     AWf G -> *)
+(*     AWTermT G a -> *)
+(*     ATMono a -> *)
+(*     ACtxTSubst G a = a -> *)
+(*     AUnify G a a G. *)
+(* Proof. *)
+(*   introv wf wt mono sub. induction wt; try(solve[constructor~]). *)
+(*   (* Typed Var *) *)
+(*   apply AUnify_Typed_Var with t; auto. *)
+
+(*   (* APP *) *)
+(*   rewrite actxtsubst_expr in sub. rewrite actxsubst_app in sub. inversion sub. *)
+(*   inversion mono. inversion H2. clear H H2 H3 H4. *)
+(*   apply AUnify_App with G; auto. *)
+(*   rewrite H0. apply~ IHwt1. apply ATrewrite actxtsubst_expr. f_equal~. *)
+(*   repeat rewrite H1. apply~ IHwt2. rewrite actxtsubst_expr. f_equal~. *)
+
+(*   (* LAM *) *)
+(*   rewrite actxtsubst_expr in sub. rewrite actxsubst_lam in sub. inversion sub. clear sub. *)
+(*   apply AUnify_Lam with (L \u dom G); auto. *)
+(*   intros y notin. *)
+(*   assert (y \notin L) by auto. *)
+(*   assert (AWf (G & y ~ AC_Var)) by apply~ AWf_Var. *)
+(*   lets: H H1. clear H. *)
+(*   lets: H0 H1 H3. clear H0. *)
+
+(*   assert(ACtxTSubst (G & y ~ AC_Var) (AT_Expr (e @@ AE_FVar y)) = *)
+(*       AT_Expr (e @@ AE_FVar y)). *)
+(*   rewrite tsubst_add_var. *)
+(*   rewrite actxtsubst_expr. f_equal. *)
+(*   rewrite~ actxsubst_open. *)
+(*   rewrite H2. rewrite actxsubst_fvar. auto. *)
+(*   lets: H H0. clear H. *)
+
+(*   rewrite tsubst_add_var in H0. *)
+(*   rewrite actxtsubst_expr in H0. *)
+(*   inversion~ H0. clear H0. *)
+(*   rewrite~ actxsubst_open in H6. *)
+(*   rewrite actxsubst_fvar in H6. *)
+
+(*   rewrite H6. auto. *)
+
+(*   (* PI *) *)
+(*   rewrite actxtsubst_expr in sub. rewrite actxsubst_pi in sub. inversion sub. clear sub. *)
+(*   apply AUnify_Pi with G (L \u dom G); auto. *)
+(*   rewrite H2. apply~ IHwt. *)
+
+(*   intros y notin. *)
+(*   assert (y \notin L) by auto. *)
+(*   assert (AWf (G & y ~ AC_Var)) by apply~ AWf_Var. *)
+(*   lets: H H1. clear H. *)
+(*   lets: H0 H1 H4. clear H0. *)
+
+(*   assert(ACtxTSubst (G & y ~ AC_Var) (t2 @@' AE_FVar y) = t2 @@' AE_FVar y). *)
+(*   rewrite tsubst_add_var. *)
+(*   rewrite~ actxtsubst_open. *)
+(*   rewrite H3. rewrite actxsubst_fvar. auto. *)
+(*   lets: H H0. clear H. *)
+
+(*   rewrite tsubst_add_var in H0. *)
+(*   rewrite~ actxtsubst_open in H0. *)
+(*   rewrite actxsubst_fvar in H0. *)
+
+(*   rewrite H0. *)
+(*   rewrite~ actxtsubst_open. *)
+(*   rewrite actxsubst_fvar. *)
+(*   rewrite H0. auto. *)
+
+(*   (* CASTUP *) *)
+(*   apply AUnify_CastUp. *)
+(*   apply~ IHwt. *)
+(*   rewrite actxtsubst_expr in sub. rewrite actxsubst_castup in sub. inversion~ sub. *)
+(*   rewrite actxtsubst_expr. f_equal. *)
+(*   repeat rewrite~ H0. *)
+
+(*   (* CASTDOWN *) *)
+(*   apply AUnify_CastDn. *)
+(*   apply~ IHwt. *)
+(*   rewrite actxtsubst_expr in sub. rewrite actxsubst_castdn in sub. inversion~ sub. *)
+(*   rewrite actxtsubst_expr. f_equal. *)
+(*   repeat rewrite~ H0. *)
+
+(*   (* ANN *) *)
+(*   rewrite actxtsubst_expr in sub. rewrite actxsubst_ann in sub. inversion sub. *)
+(*   apply AUnify_Ann with G; auto. *)
+(*   rewrite H0. apply~ IHwt1. rewrite actxtsubst_expr. f_equal~. *)
+(*   repeat rewrite H1. apply~ IHwt2. *)
+
+(*   (* FORALL *) *)
+(*   rewrite actxtsubst_expr in sub. rewrite actxsubst_forall in sub. inversion sub. clear sub. *)
+(*   apply AUnify_Forall with (L \u dom G); auto. *)
+(*   intros y notin. *)
+(*   assert (y \notin L) by auto. *)
+(*   assert (AWf (G & y ~ AC_Var)) by apply~ AWf_Var. *)
+(*   lets: H H1. clear H. *)
+(*   lets: H0 H1 H3. clear H0. *)
+
+(*   assert(ACtxTSubst (G & y ~ AC_Var) (AT_Expr (e @@ AE_FVar y)) = *)
+(*       AT_Expr (e @@ AE_FVar y)). *)
+(*   rewrite tsubst_add_var. *)
+(*   rewrite actxtsubst_expr. f_equal. *)
+(*   rewrite~ actxsubst_open. *)
+(*   rewrite H2. rewrite actxsubst_fvar. auto. *)
+(*   lets: H H0. clear H. *)
+
+(*   rewrite tsubst_add_var in H0. *)
+(*   rewrite actxtsubst_expr in H0. *)
+(*   inversion~ H0. clear H0. *)
+(*   rewrite~ actxsubst_open in H6. *)
+(*   rewrite actxsubst_fvar in H6. *)
+
+(*   rewrite H6. auto. *)
